

# Understanding Analysis, 2nd Edition: Stephen Abbott

## Chapter 2 - Section 2.3

1. Let  $x_n \geq 0$  for all  $n \in \mathbb{N}$ .

(a) If  $(x_n) \implies 0$ , show that  $(\sqrt{x_n}) \implies 0$ .

(b) If  $(x_n) \implies x$ , show that  $(\sqrt{x_n}) \implies \sqrt{x}$ .

**Solution:** Note that we *cannot* use either the algebraic or order limit theorem here, because they require that *both limits exist*. In this problem, the existence of  $\lim \sqrt{x_n}$  is what we need to prove in this first place!

With that out of the way, we need to fall back to good ol' epsilon-delta proof.

(a) We need to prove that for any  $\epsilon > 0$ , there exists  $N$  such that  $n \geq N \implies |\sqrt{x_n}| < \epsilon$ . We can discard the abs sign since  $x \geq 0$  and sqrt is non-negative.

We know  $(x_n) \implies 0$  so we can pick  $N$  such that  $x_n < \epsilon^2$  which'd make  $\sqrt{x_n} < \epsilon$ .

(b) We need  $N$  such that  $|\sqrt{x_n} - \sqrt{x}| < \epsilon$ .

We want  $|x_n - x|$  to appear so let's rationalize :  $|\frac{x_n - x}{\sqrt{x_n} + \sqrt{x}}| < \epsilon$ .

As is common in epsilon-delta proof, we can use inequalities to discard terms and simplify expressions. In this case, we're given  $x_n \geq 0$  for all  $n$  so we have

$$|\frac{x_n - x}{\sqrt{x_n} + \sqrt{x}}| \leq |\frac{x_n - x}{\sqrt{x}}| < \epsilon.$$

Since we're given  $(x_n) \implies x$  we can make  $|x_n - x|$  as small as we want, so let's pick  $N$  such that  $n \geq N \implies |x_n - x| < \epsilon\sqrt{x}$ , so we have  $\frac{x_n - x}{\sqrt{x}} < (\frac{\epsilon\sqrt{x}}{\sqrt{x}} = \epsilon)$ , as needed.

Note that this is only valid if  $x \neq 0$ , but the case  $x = 0$  has been handled in part (a).

2. Using only the definition of convergence, prove that if  $(x_n) \Rightarrow 2$ , then

(a)  $(\frac{2x_n-1}{3}) \Rightarrow 1$ ;

(b)  $(1/x_n) \Rightarrow 1/2$ .

**Solution:**

(a) We need  $|\frac{2(x_n-2)}{3}| < \epsilon$ . Pick  $n \geq N$  such that  $|x_n - 2| < \frac{3\epsilon}{2}$ .

(b) TODO.

3. **(Squeeze Theorem)**. Show that if  $x_n \leq y_n \leq z_n$  for all  $n \in \mathbf{N}$  and if  $\lim x_n = \lim z_n = l$ , then  $\lim y_n = l$  as well.

**Solution:** Just like problem 1, we can't use the algebraic or order limit theorem because it requires that  $\lim y_n$  exist, which is what we're trying to prove.

Intuitively, we can pick an  $N$  that works for both  $(x_n)$  and  $(z_n)$  simultaneously and it should work for  $(y_n)$  as well. Visualize it: either both  $(x_n)$  and  $(z_n)$  are to one side of  $l$ , or  $(x_n)$  is to the left and  $z_n$  to the right. Either case,  $(y_n)$  will also be in the  $\epsilon$  neighborhood of  $l$ .

To put it more formally, pick  $N$  that satisfies both  $x$  and  $z$ , then  $|y - l| \leq \max(|x - l|, |z - l|) < \epsilon$ .

The proof in Wikipedia is also nice.

4. Let  $(a_n) \Rightarrow 0$  and use the Algebraic Limit Theorem to compute each of the following limits (assuming the fractions are always defined):

(a)  $\lim \frac{1+2a_n}{1+3a_n-4a_n^2}$ .

(b)  $\lim \frac{(a_n+2)^2-4}{a_n}$ .

(c)  $\lim \frac{\frac{2}{a_n}+3}{\frac{1}{a_n}+5}$ .

**Solution:**

(a) 1.

(b) Simplify to  $\frac{a_n^2+4a_n}{a_n} = a_n + 4$ , then the limit is 4.

(c)  $\lim \frac{\frac{2}{a_n}+3}{\frac{1}{a_n}+5}$ .

(d) 2.

5. Let  $(x_n)$  and  $(y_n)$  be given, and define  $(z_n)$  to be the "shuffled" sequence  $(x_1, y_1, x_2, y_2, \dots, x_n, y_n, \dots)$ . Prove that  $(z_n)$  is convergent if and only if  $(x_n)$  and  $(y_n)$  are both convergent with  $\lim x_n = \lim y_n$ .

**Solution:** The problem statement doesn't say it, but we can actually prove that  $(z_n)$  converges to the same limit as  $(x_n)$  and  $(y_n)$ .

Let's prove the "if" part first: if  $(x_n)$  and  $(y_n)$  converges to the same limit then  $(z_n)$  is convergent. Pick an  $N_{xy}$  that works for both  $(x_n)$  and  $(y_n)$ , then let  $N_z = 2N_{xy}$ .

The other direction is similar. We want to prove that if  $(z_n)$  is convergent then  $(x_n)$  and  $(y_n)$  converge to the same limit. Pick an  $N_z$  for  $(z_n)$ . This  $N_z$  immediately works for both  $(x_n)$  and  $(y_n)$ , since it covers all the  $y_n$  where  $n \geq \text{floor}(N_z/2)$  in  $(z_n)$ . Similarly for  $(x_n)$ .

6. (TODO again). The answer is -1, but try to redo it next time.
7. Give an example or state that the request is impossible by referencing the proper theorem(s):
- (a) sequences  $(x_n)$  and  $(y_n)$  which both diverge but whose sum  $(x_n + y_n)$  converges.
  - (b) sequences  $(x_n)$  and  $(y_n)$  where  $(x_n)$  converges,  $(y_n)$  diverges, and  $(x_n + y_n)$  converges.
  - (c) a convergent sequence  $(b_n)$  with  $b_n \neq 0$  for all  $n$  such that  $(1/b_n)$  diverges.
  - (d) an unbounded sequence  $(a_n)$  and a convergent sequence  $(b_n)$  with  $(a_n - b_n)$  bounded.
  - (e) two sequences  $(a_n)$  and  $(b_n)$  where  $(a_n b_n)$  and  $(a_n)$  converge but  $(b_n)$  does not.

**Solution:**

(a)  $(x_n) = 1, -1, 1, -1, \dots$  and  $(y_n) = -1, 1, -1, 1, \dots$ . Then  $(x_n + y_n) = 0, 0, 0, \dots$

- (b) This is impossible. Intuitively, if  $(x_n)$  converges, then for  $(x_n + y_n)$  to also converge then  $x_n$  can only be "bumped" by something that's also convergent and not randomly by a divergent sequence.

Formally, we'll prove that if  $(x_n)$  and  $(x_n + y_n)$  converge then  $(y_n)$  must be convergent (or in logic speak, let the statement that a sequence is convergent have a truth value "True", then we want to prove "a and not b and c" is false by proving that "(a and c) implies b").

Let  $z_n = (x_n + y_n)$ , then  $\lim y_n = \lim z_n + -x_n = \lim(z_n) + -1 * \lim(x_n)$ . So by the algebraic limit theorem,  $\lim y_n$  exists.

- (c) It's tempting to say that by the algebraic division theorem, this is impossible. But note that the theorem applies only when  $\lim b_n \neq 0$ .

Consider  $(b_n) = 1, 1/2, 1/3, \dots$ . The limit is 0, but  $(1/b_n) = 1, 2, 3, \dots$  diverges.

- (d) Impossible. By theorem 2.3.2, every convergent sequence is bounded, so  $(b_n)$  is bounded. Since  $(a_n) = (a_n - b_n) + (b_n)$  and the sum of the bounds of the RHS must be a bound for  $(a_n)$  as well.

- (e) This is the reverse of part (c). Let  $(a_n) = 1, 1/2, 1/3, \dots$  and  $(b_n) = 1, 2, 3, \dots$ . Then  $(a_n b_n) = 1, 1, 1, \dots$

8. Let  $(x_n) \Rightarrow x$  and let  $p(x)$  be a polynomial.

- (a) Show  $p(x_n) = p(x)$ .
- (b) Find an example of a function  $f(x)$  and a convergent sequence  $(x_n) \Rightarrow x$  where the sequence  $f(x_n)$  converges, but not to  $f(x)$ .

**Solution:**

- (a)  $p(x_n) = \sum_{i=0}^m a_i x_n^i$  for a polynomial of degree  $m$ . We can apply the algebraic limit theorem:  $\lim a_i x_n^i = a_i \lim(x_n) \lim(x_n) \dots (i \text{ times}) = a_i x^i$ .
- (b) Although the book hasn't touched the concept of continuity at this point, but we just need to make the  $f$  discontinuous at  $x$ . For example, let  $(x_n) = 1/n$ , this sequence converges to 0. Now we make  $f(0)$  discontinuous. For example,  $f(y) = 1$  if  $y \neq 0$  else 0.  $f$  converges to 1, but  $f(0) = 0$ .

9. (a) Let  $(a_n)$  be a bounded (not necessarily convergent) sequence, and assume  $\lim b_n = 0$ . Show that  $\lim(a_nb_n) = 0$ . Why are we not allowed to use the Algebraic Limit Theorem to prove this?
- (b) Can we conclude anything about the convergence of  $(a_nb_n)$  if we assume that  $(b_n)$  converges to some nonzero limit  $b$ ?
- (c) Use (a) to prove Theorem 2.3.3, part (iii), for the case when  $a = 0$ .

**Solution:**

- (a) We need  $|a_nb_n| < \epsilon$ . Let  $B$  be a bound of  $(a_n)$ , then  $|a_nb_n| \leq |B||b_n|$ . Since we have  $\lim b_n = 0$ , we make  $|b_n| < \frac{\epsilon}{|B|}$ .

We can't use the Algebraic Limit Theorem because it requires that we know that  $(a_n)$  is convergent.

- (b) No. If we try the epsilon-delta style proof, we'll get  $|a_n(b_n - L)| + |(a_n - 1)L|$ . Unlike part (a), we can't just directly bound  $a_n - 1$ . We only know that  $a_n$  is bounded, but  $a_n - 1$  may lie outside the bound.

For a concrete counterexample, let  $(a_n) = 1, -1, 1, -1, \dots$  and  $(b_n) = 5, 5, 5, 5, \dots$

- (c) Prove the limit multiplication theorem in case  $(a_n) \implies 0$ . Well, we just need to note that convergent sequence is always bounded and directly apply part (a).